ulib/FStar.MRef.MST.fsti
@@ -1,22 +1,21 @@
 module FStar.MRef.MST
 
-open FStar.Heap
-open FStar.ST
+(*open FStar.Monotonic.Heap
 
 (* The underlying ordinary state monad of the preorder-indexed MSTATE effect *)
 
-private let st (a:Type) = heap -> M (a * heap)
+private let sti (a:Type) = heap -> M (a * heap)
 
-private let return_st (a:Type) (x:a) : st a = fun h0 -> x, h0
+private let return_sti (a:Type) (x:a) : sti a = fun h0 -> x, h0
 
-private let bind_st (a:Type) (b:Type) (f:st a) (g:a -> st b) : st b
+private let bind_sti (a:Type) (b:Type) (f:sti a) (g:a -> sti b) : sti b
           = fun (h0:heap) -> let (x,h) = f h0 in g x h
 
 total new_effect {
   MSTATE : a:Type -> Effect
-  with repr     = st
-     ; bind     = bind_st
-     ; return   = return_st
+  with repr     = sti
+     ; bind     = bind_sti
+     ; return   = return_sti
      //hiding the underlying get and put operations
 }
 
@@ -28,3 +27,4 @@ let st_post a = a -> heap -> Type0
 effect MST (a:Type) (pre:st_pre) (post: (heap -> Tot (st_post a))) =
        MSTATE a
              (fun (h0:heap) (p:(a * heap) -> Type0) -> pre h0 /\ (forall a h1. post h0 a h1 ==> p (a, h1)))
+*)
